Removed false assupmtions from memory relation definitions

tests/testMemoryModelScript.sml
@@ -2,6 +2,7 @@ open HolKernel Parse boolLib bossLib;
 load "../uvmSystemTheory";
 open uvmSystemTheory;
 open uvmMemoryModelTheory;
+open lcsymtacs;
 
 val _ = new_theory "testMemoryModel";
 
@@ -35,7 +36,7 @@ val n = Define`n m = (Int m 8)`;
 
 
 
-(* EXAMPLE 1: orderedBefore, modifiesBefore, sequencedBefore *)
+(* EXAMPLE 0: orderedBefore, modifiesBefore, sequencedBefore *)
 Define `g0= FOLDL (receive') empty
          [
             ( Write 10 0 (n 11) NOT_ATOMIC {} , 0) ;
@@ -62,7 +63,7 @@ val g0_sb0 = prove(``~sequencedBefore g0 w0_0 r0_1 ``, EVAL_TAC);
 
 
 
-(* EXAMPLE 2: sequencedBefore     (taken from POPL, p. 3) *)
+(* EXAMPLE 1: sequencedBefore     (taken from UCAM, p. 3) *)
 Define `g1'= FOLDL (receive') empty
          [                                                (* int main() {   *)
            ( Write 10 0 (n 2) NOT_ATOMIC    {} , 1 ) ;    (*   int x = 2    *)
@@ -81,9 +82,65 @@ val g1_sb1 = prove(`` sequencedBefore g1 w1_1 r1_2``,EVAL_TAC);
 val g1_sb2 = prove(`` sequencedBefore g1 w1_1 r1_3``,EVAL_TAC);
 val g1_sb3 = prove(`` sequencedBefore g1 r1_2 w1_4``,EVAL_TAC);
 val g1_sb4 = prove(`` sequencedBefore g1 r1_3 w1_4``,EVAL_TAC);
-(* readsFrom *)
-val g1_rf0 = prove( ``readsFrom g1 r1_2 w1_0``, EVAL_TAC);
-val g1_rf1 = prove( ``readsFrom g1 r1_3 w1_0``, EVAL_TAC);
+(* isReadBy *)
+val g1_rf0 = prove( ``isReadBy g1 w1_0 r1_2``, EVAL_TAC);
+val g1_rf1 = prove( ``isReadBy g1 w1_0 r1_3``, EVAL_TAC);
+
+
+(* Example 2: Data Race      (taken from UCAM, p. 3) *)
+Define `g2 = FOLDL (receive') empty
+         [                                                (* int main() {   *)
+           ( Write 10 0 (n 2) NOT_ATOMIC    {} , 1 ) ;    (*   int x = 2    *)
+           ( Write 10 1 (n 3) NOT_ATOMIC    {} , 2 ) ;    (*   {{{ x = 3    *)
+           ( Read  10 2       NOT_ATOMIC    {} , 3 )      (*   ||| x?       *)
+         ]`;                                              (*   }}}          *)
+Define `w2_0 = (EL 0 g2.nodes)`; Define `w2_1 = (EL 1 g2.nodes)`; Define `r2_2 = (EL 2 g2 .nodes)`;
+val g2_datarace = prove(
+    ``dataRace g2 w2_1 r2_2``,
+        rw [dataRace_def] THENL [
+            EVAL_TAC,
+            EVAL_TAC,
+            EVAL_TAC,
+            rw [happensBefore_def] THENL [
+                EVAL_TAC,
+                rw [Once ithb_cases] THENL [
+                    EVAL_TAC,
+                    rw [Once dob_cases] >> EVAL_TAC,
+                    rw [carriesDependencyTo_def,orderedBefore_def] >> EVAL_TAC,
+                    cheat, (* ithb - how can I Cases_on 'X'? *)
+                    cheat (* ithb *)
+                    ]
+                ],
+            rw[ happensBefore_def] THENL [
+                EVAL_TAC,
+                cheat (* ithb *)
+                ]
+            ]
+);
+
+
+
+
+(* EXAMPLE 3: sequencedBefore     (taken from UCAM, p. 3) *)
+(*Define `g= FOLDL (receive') empty
+         [                                                (* int main() {   *)
+           ( Write 10 0 (n 2) NOT_ATOMIC    {} , 1 ) ;    (*   int x = 2    *)
+           ( Write 20 1 (n 0) NOT_ATOMIC    {} , 1 ) ;    (*   int y = 0    *)
+           ( Read  10 2       NOT_ATOMIC    {} , 1 ) ;    (*   y = (x == x) *)
+           ( Read  10 3       NOT_ATOMIC    {} , 1 ) ;
+           ( Write 20 4 (n 1) NOT_ATOMIC {2;3} , 1 )
+         ]`;                                          (*   return 0;    *)
+Define `w1_0 = (EL 0 g1'.nodes)`; Define `w1_1 = (EL 1 g1'.nodes)`; Define `r1_2 = (EL 2 g1'.nodes)`;
+Define `r1_3 = (EL 3 g1'.nodes)`; Define `w1_4 = (EL 4 g1'.nodes)`;
+Define `g1'' = resolve' g1'  r1_2 w1_0`;
+Define `g1   = resolve' g1'' r1_3 w1_0`;*)
+
+
+
+
+
+
+
 
 
 (* releaseSequenceOf *)
@@ -117,7 +174,7 @@ val sw_rel0 = prove(`` sequencedBefore  g5 w5_0 w5_1 ``, EVAL_TAC );
 val sw_rel1 = prove(`` synchronizesWith g5 w5_1 r5_2 ``,
     RW_TAC (srw_ss()) [synchronizesWith_def] THEN
     `isRelease w5_1 ∧ isAcquire r5_2 ∧ sameAddress w5_1 r5_2` by EVAL_TAC THEN
-    `readsFrom g5 r5_2 w5_1 ∧ inReleaseSequenceOf g5 w5_1 w5_1` by EVAL_TAC THEN
+    `isReadBy g5 r5_2 w5_1 ∧ inReleaseSequenceOf g5 w5_1 w5_1` by EVAL_TAC THEN
     METIS_TAC []);
 val sw_rel2 = prove(`` sequencedBefore  g5 r5_2 r5_3 ``, EVAL_TAC );
 val sw_rel4 = prove(``(happensBefore g5 w5_0 r5_3)``,
@@ -236,32 +293,6 @@ val cg4_rel1 = prove(
 *)
 
 (* }}} *)
-
-
-
-
-
-
-
-(* Relations for UNDEFINED BEHAVIOUR *)
-val dataRace_def = Define`
-    dataRace g A B = (
-      ~(sameThread A B)              ∧
-       (sameAddress A B)            ∧
-       ( (isStore A) ∨ (isStore B) ) ∧
-      ~(happensBefore g A B)         ∧
-      ~(happensBefore g B A)
- )`;
-
-(* not possible in uvm-ir? *)
-val unsequencedRace_def = Define`
-    unsequencedRace g A B = (
-       (sameThread A B)              ∧
-       (sameAddress A B)             ∧
-       ( (isStore A) ∨ (isStore B) ) ∧
-      ~(sequencedBefore g A B)       ∧
-      ~(sequencedBefore g B A)
-)`;
 
 
 
